concurrency/puretree.v
@@ -5,6 +5,255 @@ Import ListNotations.
 
 Local Open Scope Z_scope.
 
+(* ranges *)
+Inductive number : Type :=
+ | Finite_Integer (n : Z)
+ | Neg_Infinity
+ | Pos_Infinity.
+
+Definition min_number a b : number :=
+ match a with
+ | Finite_Integer a1 => match b with
+                                          | Finite_Integer b1 => Finite_Integer (Z.min a1 b1)
+                                          | Neg_Infinity => b
+                                          | Pos_Infinity => a
+                                          end
+ | Neg_Infinity => a
+ | Pos_Infinity => b
+ end.
+
+Definition max_number a b : number :=
+ match a with
+ | Finite_Integer a1 => match b with
+                                          | Finite_Integer b1 => Finite_Integer (Z.max a1 b1)
+                                          | Neg_Infinity => a
+                                          | Pos_Infinity => b
+                                          end
+ | Neg_Infinity => b
+ | Pos_Infinity => a
+ end.
+
+Lemma min_min_number: forall a b, min_number a (min_number a b) = min_number a b.
+Proof.
+  intros. destruct a, b; simpl; try rewrite Z.min_id; auto. f_equal.
+  destruct (Z.min_dec n n0); rewrite e; try rewrite Z.min_id; easy.
+Qed.
+
+Lemma max_max_number: forall a b, max_number a (max_number a b) = max_number a b.
+Proof.
+  intros. destruct a, b; simpl; try rewrite Z.max_id; auto. f_equal.
+  destruct (Z.max_dec n n0); rewrite e; try rewrite Z.max_id; easy.
+Qed.
+
+Lemma min_number_comm : forall a b, min_number a b = min_number b a.
+Proof.
+  destruct a, b; auto; simpl.
+  rewrite Z.min_comm; auto.
+Qed.
+
+Lemma max_number_comm : forall a b, max_number a b = max_number b a.
+Proof.
+  destruct a, b; auto; simpl.
+  rewrite Z.max_comm; auto.
+Qed.
+
+Lemma min_number_assoc : forall a b c, min_number a (min_number b c) = min_number (min_number a b) c.
+Proof.
+  destruct a, b, c; auto; simpl.
+  rewrite Z.min_assoc; reflexivity.
+Qed.
+
+Lemma max_number_assoc : forall a b c, max_number a (max_number b c) = max_number (max_number a b) c.
+Proof.
+  destruct a, b, c; auto; simpl.
+  rewrite Z.max_assoc; reflexivity.
+Qed.
+
+Definition less_than_equal a b: bool :=
+    match a with
+ | Finite_Integer a1 => match b with
+                                          | Finite_Integer b1 => (a1 <=? b1)
+                                          | Neg_Infinity => false
+                                          | Pos_Infinity => true
+                                          end
+ | Neg_Infinity => true
+ | Pos_Infinity => match b with
+                                  | Pos_Infinity => true
+                                  | _ => false
+                                  end
+ end.
+
+Definition less_than a b: bool :=
+    match a with
+ | Finite_Integer a1 => match b with
+                                          | Finite_Integer b1 => (a1 <? b1)
+                                          | Neg_Infinity => false
+                                          | Pos_Infinity => true
+                                          end
+ | Neg_Infinity => match b with
+                                          | Neg_Infinity => false
+                                          | _ => true
+                                          end
+ | Pos_Infinity => false
+ end.
+
+Definition range := (number * number)%type.
+
+Definition range_incl (r1 r2 : range) : bool :=
+  match r1, r2 with (a1,a2), (b1,b2) => less_than_equal b1 a1 && less_than_equal a2 b2 end.
+
+Definition key_in_range (k : Z) (r : range) : bool :=
+ match r with (a1, a2) => less_than a1 (Finite_Integer k) && less_than (Finite_Integer k)  a2 end.
+
+Definition merge_range (a b : range) : range :=
+  match a, b with (a1,a2), (b1, b2) => (min_number a1 b1, max_number a2 b2) end.
+
+Lemma merge_assoc: forall a b c, merge_range (merge_range a b) c = merge_range a (merge_range b c ).
+Proof.
+  intros; unfold merge_range.
+  destruct a, b, c.
+  rewrite min_number_assoc, max_number_assoc; reflexivity.
+ Qed.
+
+Lemma merge_comm: forall a b , merge_range a b = merge_range b a .
+Proof.
+  intros; unfold merge_range.
+  destruct a, b.
+  rewrite min_number_comm, max_number_comm; reflexivity.
+Qed.
+
+ Lemma merge_id: forall a, merge_range a a = a.
+Proof.
+  intros; unfold merge_range.
+  destruct a.
+  destruct n, n0; auto; simpl; rewrite ?Z.min_id, ?Z.max_id; reflexivity.
+Qed.
+
+Lemma merge_again: forall a b c, merge_range a b = c -> merge_range a c = c.
+Proof.
+   intros. destruct a, b, c. unfold merge_range in *. inversion H; subst.
+   rewrite min_min_number. rewrite max_max_number. easy.
+ Qed.
+
+Lemma leq_min_number: forall a b, less_than_equal (min_number a b) a = true.
+Proof. intros. destruct a, b; simpl; auto; rewrite Z.leb_le; lia. Qed.
+
+Lemma leq_max_number: forall a b, less_than_equal a (max_number a b) = true.
+Proof. intros. destruct a, b; simpl; auto; rewrite Z.leb_le; lia. Qed.
+
+Lemma merge_range_incl: forall a b c,
+    merge_range a b = c -> range_incl a c = true.
+Proof.
+  intros. destruct a, b, c. unfold merge_range in H. inversion H; subst.
+  simpl. rewrite Bool.andb_true_iff. split; [apply leq_min_number | apply leq_max_number].
+Qed.
+
+Lemma merge_infinity : forall r, merge_range r (Neg_Infinity, Pos_Infinity) = (Neg_Infinity, Pos_Infinity).
+Proof.
+  destruct r; unfold merge_range, min_number, max_number.
+  destruct n, n0; auto.
+Qed.
+
+Lemma leq_min_number1: forall a b, less_than_equal (min_number a b) b = true.
+Proof. intros. destruct a, b; simpl; auto; rewrite Z.leb_le; lia. Qed.
+
+Lemma leq_max_number1: forall a b, less_than_equal b (max_number a b) = true.
+Proof. intros. destruct a, b; simpl; auto; rewrite Z.leb_le; lia. Qed.
+
+Lemma leq_entail_min_number: forall a b, less_than_equal a b = true -> a = min_number a b.
+Proof.
+intros. destruct a, b; simpl; auto;simpl in H. apply Z.leb_le in H. rewrite  Z.min_l. auto. auto. discriminate. discriminate. discriminate.
+Qed.
+
+Lemma leq_entail_max_number: forall a b, less_than_equal b a = true -> a = max_number a b.
+Proof.
+intros. destruct a, b; simpl; auto;simpl in H. apply Z.leb_le in H. rewrite  Z.max_l. auto. auto. discriminate. discriminate. discriminate.
+Qed.
+
+Lemma merge_range_incl' : forall a b, range_incl a b = true -> merge_range a b = b.
+Proof.
+  destruct a, b; simpl in *; intros.
+  apply Bool.andb_true_iff in H as [].
+  rewrite -> min_number_comm, <- leq_entail_min_number by auto.
+  rewrite -> max_number_comm, <- leq_entail_max_number by auto; auto.
+Qed.
+
+Lemma less_than_equal_trans : forall a b c, less_than_equal a b = true -> less_than_equal b c = true -> less_than_equal a c = true.
+Proof.
+  destruct a, b, c; auto; try discriminate; simpl; lia.
+Qed.
+
+Lemma range_incl_trans : forall a b c, range_incl a b = true -> range_incl b c = true -> range_incl a c = true.
+Proof.
+  destruct a, b, c; intros; simpl in *.
+  rewrite -> Bool.andb_true_iff in *.
+  destruct H, H0; split; eapply less_than_equal_trans; eauto.
+Qed.
+
+Lemma less_than_equal_less_than_trans: forall a b c, less_than_equal a b = true ->  less_than b c = true -> less_than a c = true .
+Proof.
+  destruct a, b, c; auto; try discriminate; simpl; lia.
+Qed.
+
+Lemma less_than_less_than_equal_trans: forall a b c,
+    less_than a b = true -> less_than_equal b c = true -> less_than a c = true .
+Proof.
+  destruct a, b, c; auto; try discriminate; simpl; lia.
+Qed.
+
+Lemma less_than_irrefl: forall a, less_than a a = false.
+Proof. intros. destruct a; simpl; auto. apply Z.ltb_irrefl. Qed.
+
+Lemma less_than_trans: forall a b c, less_than a b = true ->  less_than b c = true -> less_than a c = true .
+Proof.
+  destruct a, b, c; auto; try discriminate; simpl; lia.
+Qed.
+
+Lemma less_than_equal_refl: forall a, less_than_equal a a = true.
+Proof.
+  destruct a; auto; simpl; lia.
+Qed.
+
+Lemma range_incl_refl : forall r, range_incl r r = true.
+Proof.
+  destruct r; simpl.
+  rewrite !less_than_equal_refl; reflexivity.
+Qed.
+
+Lemma less_than_to_less_than_equal: forall a b, less_than a b = true -> less_than_equal a b = true.
+Proof.
+  destruct a, b; auto; simpl; lia.
+Qed.
+
+Lemma less_than_equal_antisym : forall a b, less_than_equal a b = true -> less_than_equal b a = true -> a = b.
+Proof.
+  destruct a, b; auto; try discriminate; simpl; intros.
+  f_equal; lia.
+Qed.
+
+Lemma range_incl_antisym : forall a b, range_incl a b = true -> range_incl b a = true -> a = b.
+Proof.
+  destruct a, b; simpl; intros.
+  apply Bool.andb_true_iff in H as [].
+  apply Bool.andb_true_iff in H0 as [].
+  f_equal; apply less_than_equal_antisym; auto.
+Qed.
+
+Lemma key_in_range_incl : forall k r r', key_in_range k r = true -> range_incl r r' = true -> key_in_range k r' = true.
+Proof.
+  unfold key_in_range, range_incl; destruct r, r'; intros.
+  apply andb_prop in H as [].
+  apply andb_prop in H0 as [].
+  rewrite Bool.andb_true_iff; split.
+  - eapply less_than_equal_less_than_trans; eauto.
+  - eapply less_than_less_than_equal_trans; eauto.
+Qed.
+
+Lemma range_incl_infty:
+  forall r, range_incl r (Neg_Infinity, Pos_Infinity) = true.
+Proof. intros. destruct r. simpl. destruct n0; now simpl. Qed.
+Global Hint Resolve range_incl_infty : core.
+
 Section TREES.
   Context { V : Type }.
   Variable default: V.
@@ -213,6 +462,58 @@ Section TREES.
       sorted_tree (insert_seq_opt b v l1 l2).
   Proof. intros. destruct b; simpl; apply insert_seq_sorted; constructor. Qed.
 
+Inductive EmptyRange (rn : range) : tree -> range -> Prop :=
+ | InEmptyTree : EmptyRange rn E rn
+ | InLeftSubTree l x v r n1 n2 : EmptyRange rn l (n1, Finite_Integer x) -> EmptyRange rn (T l x v r) (n1, n2)
+ | InRightSubTree l x v r n1 n2 :  EmptyRange rn r (Finite_Integer x, n2) -> EmptyRange rn (T l x v r) (n1, n2).
+
+Definition keys_in_range t r := forall k, In k t -> key_in_range k r = true.
+
+Lemma keys_in_range_subtrees : forall t1 t2 k v r, keys_in_range (T t1 k v t2) r -> sorted_tree (T t1 k v t2) ->
+  key_in_range k r = true /\ keys_in_range t1 (fst r, Finite_Integer k) /\ keys_in_range t2 (Finite_Integer k, snd r).
+Proof.
+  intros. inversion H0; subst. split; [|split].
+  - apply H; constructor; auto.
+  - intros ??.
+    specialize (H k0 (InLeft _ _ _ _ _ H1)).
+    apply H7 in H1.
+    unfold key_in_range in *.
+    destruct r; simpl; apply andb_prop in H as [->]; lia.
+  - intros ??.
+    specialize (H k0 (InRight _ _ _ _ _ H1)).
+    apply H8 in H1.
+    unfold key_in_range in *.
+    destruct r; simpl; apply andb_prop in H as [? H2].
+    simpl in *; rewrite H2; lia.
+Qed.
+
+Lemma in_range_infty:
+  forall t, keys_in_range t (Neg_Infinity, Pos_Infinity).
+Proof. repeat intro; auto. Qed.
+
+Lemma range_inside_range : forall r r_root t, EmptyRange r t r_root -> keys_in_range t r_root -> sorted_tree t -> range_incl r r_root = true.
+Proof.
+  intros; revert dependent r_root.
+  induction t; intros; inversion H; subst.
+  - apply range_incl_refl.
+  - apply keys_in_range_subtrees in H0 as (? & ? & ?); [|auto].
+    inversion H1; subst.
+    eapply range_incl_trans; [apply IHt1; eauto 1|].
+    unfold key_in_range in H.
+    unfold range_incl.
+    rewrite less_than_equal_refl.
+    apply less_than_to_less_than_equal.
+    apply andb_prop in H0 as [_ ->]; auto.
+  - apply keys_in_range_subtrees in H0 as (? & ? & ?); [|auto].
+    inversion H1; subst.
+    eapply range_incl_trans; [apply IHt2; eauto 1|].
+    unfold key_in_range in H.
+    unfold range_incl.
+    rewrite less_than_equal_refl, Bool.andb_true_r.
+    apply less_than_to_less_than_equal.
+    apply andb_prop in H0 as [-> _]; auto.
+Qed.
+
 End TREES.
 
 Arguments E {V}.
@@ -221,3 +522,5 @@ Arguments insert {V} x v s.
 Arguments lookup {V} default x t.
 Arguments pushdown_left {V} a bc.
 Arguments delete {V} x s.
+
+Global Hint Resolve in_range_infty : core.
